compcomp/BuiltinEffects.v
@@ -1,0 +1,107 @@
+Require Import Events.
+Require Import Memory.
+Require Import Coqlib.
+Require Import compcert.common.Values.
+Require Import Maps.
+Require Import Integers.
+Require Import AST.
+Require Import Globalenvs.
+Require Import Ctypes. (*for type and access_mode*)
+Require Import mem_lemmas. (*needed for definition of valid_block_dec etc*)
+
+
+Definition memcpy_Effect sz vargs m:=
+       match vargs with 
+          Vptr b1 ofs1 :: Vptr b2 ofs2 :: nil =>
+          fun b z => eq_block b b1 && zle (Int.unsigned ofs1) z &&
+                     zlt z (Int.unsigned ofs1 + sz) && valid_block_dec m b
+       | _ => fun b z => false
+       end.
+      
+Lemma memcpy_Effect_unchOn: forall m bsrc osrc sz bytes bdst odst m'
+        (LD: Mem.loadbytes m bsrc (Int.unsigned osrc) sz = Some bytes)
+        (ST: Mem.storebytes m bdst (Int.unsigned odst) bytes = Some m')
+        (SZ: sz >= 0),
+    Mem.unchanged_on
+      (fun b z=> memcpy_Effect sz (Vptr bdst odst :: Vptr bsrc osrc :: nil) 
+                 m b z = false) m m'.
+Proof. intros.
+  split; intros.
+    unfold Mem.perm. rewrite (Mem.storebytes_access _ _ _ _ _ ST). intuition.
+  unfold memcpy_Effect in H.
+    rewrite (Mem.storebytes_mem_contents _ _ _ _ _ ST).
+    destruct (valid_block_dec m b); simpl in *. rewrite andb_true_r in H; clear v.
+    destruct (eq_block b bdst); subst; simpl in *.
+      rewrite PMap.gss. apply Mem.setN_other.
+      intros. intros N; subst. 
+        rewrite (Mem.loadbytes_length _ _ _ _ _ LD), nat_of_Z_eq in H1; trivial.
+          destruct (zle (Int.unsigned odst) ofs); simpl in *.
+            destruct (zlt ofs (Int.unsigned odst + sz)). inv H.
+            omega. omega.
+    clear H. rewrite PMap.gso; trivial.
+  elim n. eapply Mem.perm_valid_block; eassumption.
+Qed.
+
+Lemma external_call_memcpy_unchOn:
+    forall {F V:Type} (ge : Genv.t F V) m ty b1 ofs1 b2 ofs2 m' a tr vres,
+    external_call (EF_memcpy (sizeof ty) a) ge 
+                  (Vptr b1 ofs1 :: Vptr b2 ofs2 :: nil) m tr vres m' -> 
+    Mem.unchanged_on
+      (fun b z=> memcpy_Effect (sizeof ty) (Vptr b1 ofs1 :: Vptr b2 ofs2 :: nil) 
+                 m b z = false) m m'.
+Proof. intros. inv H.
+  eapply memcpy_Effect_unchOn; try eassumption. omega.
+Qed.
+ 
+Lemma memcpy_Effect_validblock:
+    forall {F V:Type} (ge : Genv.t F V) m sz vargs b z,
+    memcpy_Effect sz vargs m b z = true ->
+    Mem.valid_block m b.
+Proof. intros.
+ unfold memcpy_Effect in H.  
+  destruct vargs; try discriminate.
+  destruct v; try discriminate.
+  destruct vargs; try discriminate.
+  destruct v; try discriminate.
+  destruct vargs; try discriminate.
+  destruct (valid_block_dec m b); simpl in *. trivial. 
+  rewrite andb_false_r in H. inv H. 
+Qed.
+                                                          
+Definition BuiltinEffect  {F V: Type} (ge: Genv.t F V) (ef: external_function)
+          (vargs:list val) (m:mem): block -> Z -> bool :=
+  match ef with
+    EF_memcpy sz a => memcpy_Effect sz vargs m
+  | _ => fun b z => false
+  end.
+
+Lemma BuiltinEffect_unchOn:
+    forall {F V:Type} ef (g : Genv.t F V) vargs m t vres m',
+    external_call ef g vargs m t vres m' -> 
+    Mem.unchanged_on
+      (fun b z=> BuiltinEffect g ef vargs m b z = false) m m'.
+Proof. intros.
+  destruct ef.
+    admit. (*case EF_external*)
+    admit. (*case EF_builtin*)
+    admit. (*case EF_vload*)
+    admit. (*case EF_vstore*)
+    admit. (*case EF_vload_global*)
+    admit. (*case EF_vstore_global*)
+    admit. (*case EF_malloc*)
+    admit. (*case EF_free*)
+    simpl. (*case EE_memcpy*)
+           inv H. clear - H1 H6 H7.
+           eapply memcpy_Effect_unchOn; try eassumption. omega.
+    admit. (*case EF_annot1*)
+    admit. (*case EF_annot2*)
+    admit. (*case EF_inline_asm*)
+Qed.
+
+Lemma BuiltinEffect_valid_block:
+    forall {F V:Type} ef (g : Genv.t F V) vargs m b z,
+     BuiltinEffect g ef vargs m b z = true -> Mem.valid_block m b. 
+Proof. intros. unfold BuiltinEffect in H. 
+  destruct ef; try discriminate.
+    eapply memcpy_Effect_validblock; eassumption.
+Qed.
