Makefile
@@ -121,7 +121,7 @@ LINKING_FILES= \
   #dep_linking_proof.v 
 
 COMPCOMP_FILES= \
-  Ordered.v Switch.v val_casted.v \
+  Ordered.v Switch.v val_casted.v BuiltinEffects.v\
   Clight_coop.v Clight_eff.v SimplLocals.v SimplLocalsproofEFF.v \
   Cminor.v Cminor_coop.v Cminor_eff.v \
   Csharpminor.v Csharpminor_coop.v Csharpminor_eff.v \
